LL1/Proofs/Parser/Monotonicity.v
@@ -6,6 +6,7 @@ Require Import Lib.Grammar.
 Require Import Lib.ParseTree.
 Require Import Lib.Tactics.
 
+Require Import LL1.Derivation.
 Require Import LL1.Parser.
 Require Import LL1.ParseTable.
 Require Import LL1.Proofs.Lemmas.
