LL1/Proofs/Parser/SoundnessNoFuel.v
@@ -1,0 +1,277 @@
+Require Import List.
+Require Import Omega.
+Require Import String.
+Require Import Lib.Grammar.
+Require Import Lib.ParseTree.
+Require Import Lib.Tactics.
+Require Import Lib.Utils.
+Require Import LL1.Derivation.
+Require Import LL1.Parser.
+Require Import LL1.ParseTable.
+Require Import LL1.ParseTableGen.
+Import ListNotations.
+
+Lemma p2_eq_body :
+  forall tbl sym input vis a,
+    p2 tbl sym input vis a = 
+  match (sym, input) with
+  | (T _, nil) => inl (Reject "input exhausted" input)
+  | (T y, token :: input') =>
+    if string_dec y token then
+      inr (Leaf y, input')
+    else
+      inl (Reject "token mismatch" input)
+  | (NT x, _) =>
+    match ptlk_dec x (peek input) tbl with
+    | inl _ => inl (Reject "lookup failure" input)
+    | inr (exist _ gamma Hlk) =>
+      match List.in_dec NT_as_DT.eq_dec x vis with
+      | left _ => inl (LeftRec x vis input)
+      | right Hnin => 
+        match pf2 tbl gamma input (x :: vis) (hole1 _ _ _ _  _ _ _ a Hlk Hnin) with
+        | inl pfail => inl pfail
+        | inr (sts, input') =>
+          inr (Node x sts, input')
+        end
+      end
+    end
+  end.
+Proof.
+  intros; simpl; destruct a; cr.
+Qed.
+
+Lemma pf2_eq_body :
+  forall tbl gamma input vis a,
+    pf2 tbl gamma input vis a =
+    match gamma as g return gamma = g -> _  with
+    | nil => fun _ => inr (nil, input)
+    | sym :: gamma' => fun Hg => 
+                         match p2 tbl sym input vis (hole2 _ _ _ _ _ a) with
+                         | inl pfail => inl pfail
+                         | inr (lSib, input') =>
+                           match Compare_dec.lt_dec (List.length input') (List.length input) with
+                           | left Hlt =>
+                             match pf2 tbl gamma' input' [] (hole3 _ _ _ _ _ _ _ a Hlt) with
+                             | inl pfail => inl pfail
+                             | inr (rSibs, input'') =>
+                               inr (lSib :: rSibs, input'')
+                             end
+                           | right Hnlt =>
+                             match pf2 tbl gamma' input vis (hole4 _ _ _ _ _ _ a Hg) with
+                             | inl pfail => inl pfail
+                             | inr (rSibs, input'') =>
+                               inr (lSib :: rSibs, input'')
+                             end
+                           end
+                         end
+    end eq_refl.
+Proof.
+  intros; simpl; destruct a; cr.
+Qed.
+
+Lemma p2_t_ret_leaf :
+  forall tbl
+         input rem
+         vis
+         y
+         (a : Acc triple_lt (meas tbl input vis (F_arg (T y))))
+         tr,
+    p2 tbl (T y) input vis a = inr (tr, rem)
+    -> isLeaf tr = true.
+Proof.
+  intros; destruct a; cr; tc.
+  inv H; auto.
+Qed.
+
+Lemma p2_nt_ret_node :
+  forall tbl
+         input rem
+         vis
+         x
+         (a : Acc triple_lt (meas tbl input vis (F_arg (NT x))))
+         tr,
+    p2 tbl (NT x) input vis a = inr (tr, rem)
+    -> isNode tr = true.
+Proof.
+  intros; destruct a; cr; tc.
+  inv H; auto.
+Qed.
+
+Lemma input_length_invariant :
+  forall (g   : grammar)
+         (tbl : parse_table),
+    parse_table_for tbl g
+    -> forall (tr        : tree)
+              (sym       : symbol)
+              (input rem : list terminal)
+              (vis       : list nonterminal)
+              (a : Acc triple_lt (meas tbl input vis (F_arg sym))),
+      p2 tbl sym input vis a = inr (tr, rem)
+      -> List.length rem < List.length input
+         \/ rem = input.
+Proof.
+  intros g tbl Htbl tr.
+  induction tr as [ s
+                  | s f IHpf
+                  |
+                  | tr IHp f IHpf ]
+                    using tree_nested_ind with
+      
+      (Q := fun f =>
+              forall (gamma : list symbol)
+                     (input rem : list string)
+                     (vis : list nonterminal)
+                     (a   : Acc triple_lt (meas tbl input vis (G_arg gamma))),
+                pf2 tbl gamma input vis a = inr (f, rem)
+                -> List.length rem < List.length input
+                   \/ rem = input); intros; destruct a.
+
+  - destruct sym as [y | x].
+    + cr; tc.
+      inv H; auto.
+    + apply p2_nt_ret_node in H; inv H.
+
+  - destruct sym as [y | x].
+    + apply p2_t_ret_leaf in H; inv H.
+    + step; tc.
+      step.
+      step; tc.
+      step_eq Hpf; tc.
+      step.
+      inv H.
+      apply IHpf in Hpf; auto.
+
+  - cr; tc.
+    inv H; auto.
+
+  - step; tc.
+    step_eq Hp; tc.
+    step.
+    step.
+    + step_eq Hpf; tc.
+      step.
+      inv H.
+      apply IHp in Hp; clear IHp.
+      apply IHpf in Hpf; clear IHpf.
+      destruct Hpf.
+      * left; omega.
+      * subst; auto.
+    + step_eq Hpf; tc.
+      step.
+      inv H.
+      apply IHpf in Hpf; clear IHpf; auto.
+Qed.
+
+Lemma p2_sound' :
+  forall (g   : grammar)
+         (tbl : parse_table),
+    parse_table_for tbl g
+    -> forall (tr        : tree)
+              (sym       : symbol)
+              (input rem : list terminal)
+              (vis       : list nonterminal)
+              (a : Acc triple_lt (meas tbl input vis (F_arg sym))),
+      p2 tbl sym input vis a = inr (tr, rem)
+      -> exists word,
+        word ++ rem = input
+        /\ (@sym_derives_prefix g) sym word tr rem.
+Proof.
+  intros g tbl Htbl tr.
+  induction tr as [ s
+                  | s f IHpf
+                  |
+                  | tr IHp f IHpf ]
+                    using tree_nested_ind with
+
+      (Q := fun f =>
+              forall (gamma : list symbol)
+                     (input rem : list string)
+                     (vis : list nonterminal)
+                     (a   : Acc triple_lt (meas tbl input vis (G_arg gamma))),
+                pf2 tbl gamma input vis a = inr (f, rem)
+                -> exists word,
+                  word ++ rem = input
+                  /\ gamma_derives_prefix gamma word f rem); intros; destruct a.
+
+  - destruct sym as [y | x].
+    + rewrite p2_eq_body in H.
+      step; tc.
+      step_eq Hbeq; tc.
+      inv H.
+      eexists; split.
+      * rewrite cons_app_singleton; auto.
+      * constructor; auto.
+    + apply p2_nt_ret_node in H; inv H.
+
+  - destruct sym as [y | x].
+    + apply p2_t_ret_leaf in H; inv H.
+    + simpl in H.
+      destruct (ptlk_dec x (peek input) tbl) as [| e]; tc.
+      destruct e as [gamma Hlk].
+      step; tc.
+      step_eq Hpf; tc.
+      step.
+      inv H.
+      apply IHpf in Hpf; clear IHpf.
+      destruct Hpf as [word [Happ Hg]]; subst.
+      eexists; split; eauto.
+      apply Htbl in Hlk; destruct Hlk.
+      econstructor; eauto.
+
+  - rewrite pf2_eq_body in H.
+    cr; tc.
+    inv H.
+    exists nil; split; auto.
+    constructor.
+
+  - rewrite pf2_eq_body in H.
+    step; tc.
+    step_eq Hp; tc.
+    step.
+    step.
+    + step_eq Hpf; tc.
+      step.
+      inv H.
+      apply IHp in Hp; clear IHp.
+      apply IHpf in Hpf; clear IHpf.
+      destruct Hp  as [wpre [Happ Hs]]; subst.
+      destruct Hpf as [wsuf [Happ Hg]]; subst.
+      exists (wpre ++ wsuf); split.
+      * rewrite app_assoc; auto.
+      * constructor; auto.
+    + pose proof Hp as Hp'.
+      eapply input_length_invariant in Hp'; eauto.
+      destruct Hp'; try contradiction.
+      subst.
+      step_eq Hpf; tc.
+      step.
+      inv H.
+      apply IHp in Hp; clear IHp.
+      apply IHpf in Hpf; clear IHpf.
+      destruct Hp as [wpre [Happ Hs]].
+      apply l_ident_eq_nil in Happ; subst.
+      destruct Hpf as [wsuf [Happ Hg]]; subst.
+      exists ([] ++ wsuf); split; auto.
+      constructor; auto.
+Qed.
+
+Lemma p2_sound :
+  forall (g   : grammar)
+         (tbl : parse_table),
+    parse_table_for tbl g
+    -> forall (tr        : tree)
+              (sym       : symbol)
+              (word rem  : list terminal)
+              (vis       : list nonterminal)
+              (a : Acc triple_lt (meas tbl (word ++ rem) vis (F_arg sym))),
+      p2 tbl sym (word ++ rem) vis a = inr (tr, rem)
+      -> (@sym_derives_prefix g) sym word tr rem.
+Proof.
+  intros g tbl Htbl tr sym word rem vis a Hp.
+  pose proof Hp as Hp'.
+  eapply p2_sound' in Hp; eauto.
+  destruct Hp as [word' [Happ Hder]].
+  apply app_inv_tail in Happ.
+  subst; auto.
+Qed.
+
