LL1/Tests/ParserTests.v
@@ -14,9 +14,4 @@ Example g311_test :
   parse g311ParseTable (NT X) g311Sentence1 100 =
   (Some g311ParseTree1, nil).
 Proof. auto. Qed.
-                
-Example xy_test :
-  parse xy_parse_table (NT X) nil 100 =
-  (Some (Node X [Node Y []]), nil).
-Proof. auto. Qed.
 
